\subsubsection{莫比乌斯反演}
	$$ \begin{aligned}
		f(n) = \sum_{d | n} g(d) \Leftrightarrow g(n) = \sum_{d | n} \mu\left( \frac n d \right) f(d) \\
		f(d) = \sum_{d | k} g(k) \Leftrightarrow g(d) = \sum_{d | k} \mu\left( \frac k d \right) f(k)
	\end{aligned} $$

\subsubsection{其他常用公式}
	$$\mu * I = e \quad (e(n) = [n = 1])$$

	$$\varphi * I = id $$

	$$\mu * id = \varphi $$

	$$\sigma_0 = I * I ,\, \sigma_1 = id * I ,\, \sigma_k = id^{k - 1} * I$$

	$$\sum_{i = 1} ^ n \left[(i, n) = 1\right] i = n \frac {\varphi(n) + e(n)} 2$$
	
	$$\sum_{i = 1} ^ n \sum_{j = 1} ^ i \left[(i, j) = d\right] = S_\varphi \left( \left\lfloor \frac n d \right\rfloor \right)$$

	$$\sum_{i = 1} ^ n \sum_{j = 1} ^ m \left[(i, j) = d\right] = \sum_{d | k} \mu\left( \frac k d \right) \left\lfloor \frac n k \right\rfloor \left\lfloor \frac m k \right\rfloor$$

	$$ \sum_{i = 1} ^ n f(i) \sum_{j = 1} ^ {\left\lfloor \frac n i \right\rfloor} g(j) = \sum_{i = 1} ^ n g(i) \sum_{j = 1} ^ {\left\lfloor \frac n i \right\rfloor} f(j) $$